examples/mw/MWB01proof.v
@@ -1,0 +1,354 @@
+Require Import HoareDef MWHeader MWB0 MWC1 SimModSem.
+Require Import Coqlib.
+Require Import ImpPrelude.
+Require Import Skeleton.
+Require Import PCM.
+Require Import ModSem Behavior.
+Require Import Relation_Definitions.
+Require Import Mem1.
+
+(*** TODO: export these in Coqlib or Universe ***)
+Require Import Relation_Operators.
+Require Import RelationPairs.
+From ITree Require Import
+     Events.MapDefault.
+From ExtLib Require Import
+     Core.RelDec
+     Structures.Maps
+     Data.Map.FMapAList.
+
+Require Import HTactics IPM ProofMode STB.
+
+Set Implicit Arguments.
+
+Local Open Scope nat_scope.
+
+
+
+
+
+Section SIMMODSEM.
+
+  Context `{Σ: GRA.t}.
+  Context `{@GRA.inG memRA Σ}.
+  Context `{@GRA.inG spRA Σ}.
+
+  Let W: Type := Any.t * Any.t.
+
+(*   Definition trans (arr: val) (i v: Z): local_state := *)
+(*     mk_lst (fun k => if dec k i then opt else normal *)
+(* Record local_state : Set := mk_lst { lst_cls : Z → cls;  lst_opt : Z → val;  lst_map : val } *)
+
+  Definition le (w0 w1: option (Any.t * Any.t)): Prop :=
+    match w0, w1 with
+    | Some w0, Some w1 => w0 = w1
+    | None, None => True
+    | _, _ => False
+    end
+  .
+
+  Global Program Instance le_PreOrder: PreOrder le.
+  Next Obligation. unfold le. ii. des_ifs. Qed.
+  Next Obligation. unfold le. ii. des_ifs. Qed.
+
+  Let wf: _ -> W -> Prop :=
+    @mk_wf
+      _
+      (option (Any.t * Any.t))
+      (fun w0 mp_src mp_tgt =>
+         ({{"UNINIT": OwnM sp_black ** ⌜(mp_src = tt↑) ∧ w0 = None ∧
+                      ∃ (idv: option (val * val)) (map: val), mp_tgt = (idv, map)↑⌝}} ∨
+          (* {{"INIT": OwnM sp_black ** ⌜w0 = None ∧ (∃ map i v cls, mp_tgt = (Some (Vint i, v), map)↑ *)
+          (*                   ∧ mp_src = (mk_lst cls (fun k => if dec k i then v else Vundef) map)↑)⌝}} ∨ *)
+          {{"INIT": OwnM sp_black ** ⌜w0 = None ∧ (∃ map idv cls, mp_tgt = (idv, map)↑
+   (* ∧ match idv with *)
+   (*   | Some (i, v) => mp_src = (mk_lst cls (fun k => if dec (Vint k) i then v else Vundef) map)↑ ∧ cls i = opt *)
+   (*   | None => mp_src = (mk_lst cls (fun _ => Vundef) map)↑ *)
+   (*   end)⌝}} ∨ *)
+   ∧ ((idv = None ∧ mp_src = (mk_lst cls (fun _ => Vundef) map)↑) ∨
+      (∃ i v, idv = Some (Vint i, v) ∧
+              mp_src = (mk_lst cls (fun k => if dec k i then v else Vundef) map)↑ ∧ cls i = opt)))⌝}} ∨
+          {{"LOCKED": OwnM sp_black ** OwnM sp_white ** ⌜w0 = Some (mp_src, mp_tgt)⌝}}
+         )%I)
+  .
+     (* | Some (i, v) => mp_src = (mk_lst cls (fun k => if dec (Vint k) i then v else Vundef) map)↑ ∧ cls i = opt *)
+     (* | None =>  *)
+
+  Theorem correct: refines2 [MWB0.MW] [MWC1.MW].
+  Proof.
+    eapply adequacy_local2. econs; ss.
+    i. econstructor 1 with (wf:=wf) (le:=le); et; swap 2 3.
+    { typeclasses eauto. }
+    { esplits; et. econs; et. eapply to_semantic. iIntros "H". ss; et. iFrame. iLeft. iSplits; ss.
+      iPureIntro. iSplits; ss; et. }
+
+    econs; ss.
+    { init. harg. fold wf. unfold mainF, MWB0.mainF, ccallU. mDesAll; des; clarify.
+      mDesOr "INV"; ss; mDesAll; des; clarify.
+      { steps. astop. steps.
+        force_l; stb_tac; ss; clarify. steps.
+        hcall _ _ (Some (_, _)) with "*".
+        { iModIntro. iSplits; ss; et. iRight. iRight. iFrame. iSplits; ss; et. }
+        { esplits; ss; et. }
+        fold wf. mDesAll; des; clarify.
+        mDesOr "INV"; mDesAll; des; clarify; ss.
+        mDesOr "INV"; mDesAll; des; clarify; ss.
+        steps.
+
+        force_l; stb_tac; ss; clarify. steps.
+        hcall _ _ None with "*".
+        { iModIntro. iSplits; ss; et. iFrame. iSplits; ss; et. iRight. iLeft. iSplits; ss; et.
+          iPureIntro. eexists _, None, _; cbn. esplits; ss; et. }
+        { esplits; ss; et. }
+        fold wf. mDesAll; des; clarify. steps. force_l; stb_tac; ss; clarify. steps.
+
+        hcall _ _ None with "*".
+        { iModIntro. iSplits; ss; et. iFrame. iSplits; ss; et. }
+        { esplits; ss; et. }
+        fold wf. mDesAll; des; clarify. steps.
+
+        hret None; ss.
+        { iModIntro. iSplits; ss; et.
+          iDes; des; clarify.
+          - iFrame; iSplits; ss; et. iLeft. iSplits; ss; et.
+          - iFrame; iSplits; ss; et. iRight. iLeft. iSplits; ss; et. iPureIntro. esplits; ss; et.
+          - iFrame; iSplits; ss; et. iRight. iLeft. iSplits; ss; et. iPureIntro. esplits; ss; et.
+            right. esplits; ss; et.
+        }
+      }
+      mDesOr "INV"; ss; cycle 1.
+      { mDesAll; des; clarify.
+        admit "ez".
+      }
+      { mDesAll; des_safe; clarify. steps. astop. steps.
+
+        force_l; stb_tac; ss; clarify. steps.
+        hcall _ _ None with "*".
+        { iModIntro. iSplits; ss; et. iFrame. iSplits; ss; et. iRight. iLeft. iSplits; ss; et.
+          iPureIntro. des; clarify; iSplits; ss; et. left. iSplits; ss; et. f_equal. }
+        { esplits; ss; et. }
+        fold wf. mDesAll; des; clarify. steps. force_l; stb_tac; ss; clarify. steps.
+
+        - 
+      }
+      mDesOr "INV"; ss; mDesAll; des; clarify.
+      - steps. astop. steps.
+        force_l; stb_tac; ss; clarify. steps.
+        hcall _ _ (Some (_, _)) with "*".
+        { iModIntro. iSplits; ss; et. iRight. iRight. iFrame. iSplits; ss; et. }
+        { esplits; ss; et. }
+        fold wf. mDesAll; des; clarify.
+        mDesOr "INV"; mDesAll; des; clarify; ss.
+        mDesOr "INV"; mDesAll; des; clarify; ss.
+        steps.
+
+        force_l; stb_tac; ss; clarify. steps.
+        hcall _ _ None with "*".
+        { iModIntro. iSplits; ss; et. iFrame. iSplits; ss; et. iRight. iLeft. iSplits; ss; et.
+          iPureIntro. eexists _, None, _; cbn. esplits; ss; et. }
+        { esplits; ss; et. }
+        fold wf. mDesAll; des; clarify. steps. force_l; stb_tac; ss; clarify. steps.
+
+        hcall _ _ None with "*".
+        { iModIntro. iSplits; ss; et. iFrame. iSplits; ss; et. }
+        { esplits; ss; et. }
+        fold wf. mDesAll; des; clarify. steps.
+
+        hret None; ss.
+        { iModIntro. iSplits; ss; et.
+          iDes; des; clarify.
+          - iFrame; iSplits; ss; et. iLeft. iSplits; ss; et.
+          - iFrame; iSplits; ss; et. iRight. iLeft. iSplits; ss; et. iPureIntro. esplits; ss; et.
+          - iFrame; iSplits; ss; et. iRight. iLeft. iSplits; ss; et. iPureIntro. esplits; ss; et.
+            right. esplits; ss; et.
+        }
+        { esplits; ss; et. }
+    }
+          -
+          iSplits; ss; et.
+          - iLeft. iSplits; ss; et.
+          - iRight. iLeft. iSplits; ss; et. iPureIntro. esplits; ss; et.
+          - iRight. iRight. iSplits; ss; et. iPureIntro. esplits; ss; et.
+          -
+          
+        - }
+        { 
+
+        mDesOr "INV"; mDesAll; des; clarify; ss; cycle 1.
+        { des_ifs.
+          mDesOr "INV"; mDesAll; des; clarify; ss.
+        }
+        mDesOr "INV"; mDesAll; des; clarify; ss.
+        steps.
+        iPureIntro. left. esplits; et.
+        hide_k. Set Printing All. rewrite Any.upcast_downcast.
+      -
+        des_u. steps. unfold mainF, MWC0.mainF, ccallU. steps. fold wf.
+      mAssert (OwnM sp_black ** OwnM sp_white ** ⌜w = None ∧ ∃ (arr map: val), mp_tgt = (arr, map)↑⌝) with "*" as "A".
+      { iDes; des; clarify; try (by iFrame; iSplits; ss; et). admit "ez". }
+      mDesAll; des; clarify.
+      astart 1. acatch. hcall _ 100 (Some (_, _)) with "*".
+      { iModIntro. iFrame. iSplits; ss; et. }
+      { esplits; ss; et. }
+      fold wf. steps. astop. mDesAll; des; clarify.
+      mDesOr "INV"; mDesAll; des; clarify; ss.
+      mDesOr "INV"; mDesAll; des; clarify; ss.
+      steps. force_l; stb_tac; ss; clarify. steps.
+      hcall _ _ _ with "-A".
+      { iModIntro. iFrame. iSplits; ss; et. }
+      { esplits; ss; et. }
+      fold wf. mDesAll; des; clarify. steps. force_l; stb_tac; ss; clarify.
+      mDesOr "INV"; mDesAll; des; clarify; ss.
+      mDesOr "INV"; mDesAll; des; clarify; ss. steps.
+      hcall _ _ _ with "*".
+      { rewrite repeat_replicate. iDestruct (OwnM_replicate_sepL with "A") as "A". iMod "A".
+        iModIntro. iSplits; ss; et. iFrame. iSplits; ss; et. iRight. iLeft. iSplits; ss; et.
+        - iPureIntro. eapply sim_init.
+      }
+      { esplits; ss; et. }
+      fold wf. mDesAll; des; clarify. steps. force_l; stb_tac; ss; clarify. steps.
+
+      hcall _ _ _ with "*".
+      { iModIntro. iFrame. iSplits; ss; et. }
+      { esplits; ss; et. }
+      fold wf. mDesAll; des; clarify. steps. ss. des_ifs.
+      hret None; ss.
+      { iModIntro. iFrame. iSplits; ss; et. }
+    }
+
+    econs; ss.
+    { init. harg. mDesAll. des; clarify. des_u.
+      assert(w = None).
+      { repeat mDesOr "INV"; mDesAll; des; clarify. mAssertPure False; ss. admit "ez". }
+      steps. unfold loopF, MWC0.loopF, ccallU. steps. fold wf.
+      force_l; stb_tac; ss; clarify. steps. hcall _ _ _ with "*".
+      { iFrame. iSplits; ss; et. }
+      { esplits; ss; et. }
+      fold wf. mDesAll; des; clarify. steps. force_l; stb_tac; ss; clarify. steps. hcall _ _ _ with "*".
+      { iFrame. iSplits; ss; et. }
+      { esplits; ss; et. }
+      fold wf. mDesAll; des; clarify. steps. ss. des_ifs.
+      hret None; ss.
+      { iModIntro. iFrame; et. }
+    }
+
+    econs; ss.
+    { init. harg. mDesAll. des; clarify. des_u. unfold putF, MWC0.putF, ccallU. steps. fold wf.
+      force_r; ss. esplits; ss. steps.
+      mDesOr "INV"; mDesAll; des; clarify.
+      { exfalso. clear - _UNWRAPU0. apply Any.downcast_upcast in _UNWRAPU0. des.
+        apply Any.upcast_inj in _UNWRAPU0. des; clarify.
+        assert(T: exists (a b: local_state), a <> b).
+        { exists (mk_lst (fun _ => uninit) (fun _ => Vundef) Vundef),
+          (mk_lst (fun _ => uninit) (fun _ => Vundef) (Vint 1)). ii. clarify. }
+        des. revert a b T. rewrite EQ. i. repeat des_u; ss.
+      }
+      mDesOr "INV"; mDesAll; des; clarify; cycle 1.
+      { mAssertPure False; ss. admit "ez". }
+      steps. rewrite Any.upcast_downcast in *. clarify. steps.
+      destruct ((0 <=? z)%Z && (z <? 100)%Z) eqn:T.
+      - inv PURE2. hexploit (SIM (Z.to_nat z)); [lia|]. rewrite ! Nat2Z.id in *;rewrite Z2Nat.id in *;try lia.
+        intro U. des; ss.
+        + rewrite INIT. ss. steps.
+          mAssert _ with "A2".
+          { iDestruct (big_sepL_insert_acc with "A2") as "[B C]"; et.
+            instantiate (1:=_ ** _). iSplitL "B". { iExact "B". } iExact "C". }
+          mDesAll; ss. rewrite Z2Nat.id in *; try lia. rewrite scale_int_8. steps.
+          astart 1. acatch. hcall _ (_, _, _) (Some (_, _)) with "-A2".
+          { iModIntro. iFrame. iSplitR "A1"; et. }
+          { esplits; ss; et. }
+          fold wf. mDesAll; des; clarify. ss. des_ifs.
+          mDesOr "INV"; mDesAll; des; clarify; ss.
+          mDesOr "INV"; mDesAll; des; clarify; ss.
+          steps. astop. steps. hret None; ss.
+          { iModIntro. iFrame. iSplits; ss; et. iRight. iLeft. iSplits; ss; et; cycle 1.
+            { iApply "A2"; et. }
+            iPureIntro. eapply sim_upd; et; try lia. econs; et.
+          }
+        + rewrite UNINIT. ss. steps. force_l. exists true. steps. unfold set; ss. des_ifs. steps.
+          mAssert _ with "A2".
+          { iDestruct (big_sepL_insert_acc with "A2") as "[B C]"; et.
+            instantiate (1:=_ ** _). iSplitL "B". { iExact "B". } iExact "C". }
+          mDesAll; ss. rewrite Z2Nat.id in *; try lia. rewrite scale_int_8. steps.
+          astart 1. acatch. hcall _ (_, _, _) (Some (_, _)) with "-A2".
+          { iModIntro. iFrame. iSplitR "A1"; et. }
+          { esplits; ss; et. }
+          fold wf. mDesAll; des; clarify. ss. des_ifs.
+          mDesOr "INV"; mDesAll; des; clarify; ss.
+          mDesOr "INV"; mDesAll; des; clarify; ss.
+          steps. astop. steps. hret None; ss.
+          { iModIntro. iFrame. iSplits; ss; et. iRight. iLeft. iSplits; ss; et; cycle 1.
+            { iApply "A2"; et. }
+            iPureIntro. eapply sim_upd2; et; try lia. econs; et.
+          }
+      - steps.
+        destruct (lst_cls l z) eqn:U.
+        + ss. steps. force_l. exists false. steps. unfold set. des_ifs. steps. force_l; stb_tac; ss; clarify.
+          steps. hcall _ _ _ with "A INIT".
+          { iModIntro. iSplits; ss; et. iRight. iRight. iFrame. iSplits; ss; et. }
+          { esplits; ss; et. }
+          fold wf. ss. des_ifs.
+          mDesOr "INV"; mDesAll; des; clarify; ss.
+          mDesOr "INV"; mDesAll; des; clarify; ss.
+          steps. hret None; ss.
+          { iSplits; ss; et. iModIntro. iFrame. iSplits; ss; et. iRight. iLeft. iSplits; ss; et.
+            iPureIntro. eapply sim_upd3; et; try lia. }
+        + exfalso. inv PURE2. hexploit (NORMAL z); et. { lia. } intro V. rewrite U in *; des; ss.
+        + ss. steps. rewrite U. ss. steps. force_l; stb_tac; ss; clarify. steps.
+          hcall _ _ _ with "-A2".
+          { iModIntro. iSplits; ss; et. iRight. iRight. iFrame. iSplits; ss; et. }
+          { esplits; ss; et. }
+          fold wf. ss. des_ifs.
+          mDesOr "INV"; mDesAll; des; clarify; ss.
+          mDesOr "INV"; mDesAll; des; clarify; ss.
+          steps. hret None; ss.
+          { iSplits; ss; et. iModIntro. iFrame. iSplits; ss; et. iRight. iLeft. iSplits; ss; et. }
+    }
+
+    econs; ss.
+    { init. harg. mDesAll. des; clarify. des_u. unfold getF, MWC0.getF, ccallU. steps. fold wf.
+      force_r. esplits; ss. steps.
+      mDesOr "INV"; mDesAll; des; clarify.
+      { exfalso. clear - _UNWRAPU1. apply Any.downcast_upcast in _UNWRAPU1. des.
+        apply Any.upcast_inj in _UNWRAPU1. des; clarify.
+        assert(T: exists (a b: local_state), a <> b).
+        { exists (mk_lst (fun _ => uninit) (fun _ => Vundef) Vundef),
+          (mk_lst (fun _ => uninit) (fun _ => Vundef) (Vint 1)). ii. clarify. }
+        des. revert a b T. rewrite EQ. i. repeat des_u; ss.
+      }
+      mDesOr "INV"; mDesAll; des; clarify; cycle 1.
+      { mAssertPure False; ss. admit "ez". }
+      steps. rewrite Any.upcast_downcast in *. clarify. steps.
+      destruct ((0 <=? z)%Z && (z <? 100)%Z) eqn:T.
+      - inv PURE2. hexploit (SIM (Z.to_nat z)); [lia|]. rewrite ! Nat2Z.id in *;rewrite Z2Nat.id in *;try lia.
+        intro U. des; ss.
+        + rewrite INIT. ss. steps.
+          mAssert _ with "A2".
+          { iDestruct (big_sepL_delete with "A2") as "[B C]"; et. xtra. }
+          mDesAll; ss. rewrite Z2Nat.id in *; try lia. rewrite scale_int_8. steps.
+          astart 1. acatch. hcall _ (_, _, _) (Some (_, _)) with "-A2".
+          { iModIntro. iFrame. iSplits; ss; et. }
+          { esplits; ss; et. }
+          fold wf. mDesAll; des; clarify. ss. des_ifs.
+          mDesOr "INV"; mDesAll; des; clarify; ss.
+          mDesOr "INV"; mDesAll; des; clarify; ss.
+          steps. astop. steps. hret None; ss.
+          { iModIntro. iFrame. iSplits; ss; et. iRight. iLeft. iSplits; ss; et; cycle 1.
+            { iApply big_sepL_delete; et. rewrite Z2Nat.id. iFrame. lia. }
+          }
+      - steps. inv PURE2. exploit (NORMAL z); et. { lia. } intro U; des; clarify. rewrite U. ss.
+        steps. force_l; stb_tac; ss; clarify. steps.
+        hcall _ _ (Some (_, _)) with "-A2".
+        { iModIntro. iFrame. iSplits; ss; et. }
+        { esplits; ss; et. }
+        fold wf. mDesAll; des; clarify. ss. des_ifs.
+        mDesOr "INV"; mDesAll; des; clarify; ss.
+        mDesOr "INV"; mDesAll; des; clarify; ss.
+        steps. hret None; ss.
+        { iModIntro. iFrame. iSplits; ss; et. iRight. iLeft. iSplits; ss; et. }
+    }
+
+  Unshelve. all: ss. all: try exact 0.
+  Qed.
+
+End SIMMODSEM.
